1. Node type in mark.c is redefined. Previous version has an error because of some changes after compcert-2.4. 2. VST is updated. Legal_alignas_type is weakened a little bit such that our node_type is legal. (While it is in fact legal in the newest compcert.) 3. VST version of trinode is proved an instance of SpatialGraphAssum type class.

data_structure/spatial_graph_VST.v
@@ -1,13 +1,14 @@
-Require Import RamifyCoq.veric_ext.SeparationLogic.
 Require Import RamifyCoq.data_structure.spatial_graph.
 Require Import RamifyCoq.msl_ext.abs_addr.
 Require Import RamifyCoq.msl_ext.seplog.
 Require Import VST.veric.SeparationLogic.
+Require Import RamifyCoq.veric_ext.SeparationLogic.
 Require Import RamifyCoq.msl_ext.alg_seplog.
 Require Import RamifyCoq.sample_mark.env_mark.
+Require Import RamifyCoq.veric_ext.SeparationLogic.
+Require Import RamifyCoq.floyd_ext.DataatSL.
 
-(* Move into env_mark. *)
-Definition node_type := (talignas 4%N (Tstruct _Node noattr)).
+Local Open Scope logic.
 
 Instance SGS_VST: SpatialGraphSetting.
   apply (Build_SpatialGraphSetting int pointer_val NullPointer PV_eq_dec).
@@ -17,4 +18,75 @@ Definition trinode (sh: share) (p: Addr) (dlr: Val): mpred :=
   match dlr with
   | (d, l, r) => data_at sh node_type (repinj node_type (d, (l, r))) (pointer_val_val p)
   end.
+
+Instance MSLstandard sh : MapstoSepLog AV_SGraph (trinode sh).
+Proof.
+  intros.
+  apply mkMapstoSepLog.
+  intros.
+  apply derives_precise with (memory_block sh (sizeof cenv_cs node_type) (pointer_val_val p));
+   [| apply memory_block_precise].
+  apply exp_left; intros [[? ?] ?].
+  unfold trinode.
+  apply data_at_memory_block.
+Defined.
+
+Instance sMSLstandard sh : StaticMapstoSepLog AV_SGraph (trinode sh).
+Proof.
+  apply mkStaticMapstoSepLog; simpl; intros.
+  + hnf in H. simpl in H. unfold addr_eqb in H. simpl in H.
+    destruct PV_eq_dec; congruence.
+  + unfold trinode.
+    destruct v1 as [[d1 l1] r1].
+    destruct v2 as [[d2 l2] r2].
+    rewrite (add_andp _ _ (data_at_compatible _ _ _ (pointer_val_val p1))).
+    rewrite (add_andp _ _ (data_at_compatible _ _ _ (pointer_val_val p2))).
+    normalize.
+    apply data_at_conflict.
+    change (sizeof cenv_cs node_type) with 16.
+    unfold addr_eqb in H; simpl in H.
+    destruct (PV_eq_dec p1 p2); [| congruence].
+    subst.
+    apply pointer_range_overlap_refl; try omega.
+    destruct H0; auto.
+  + unfold msl_ext.seplog.mapsto_, trinode.
+    eapply disj_derives with
+     (!! field_compatible node_type [] (pointer_val_val p1) &&
+        EX v: reptype node_type, data_at sh node_type v (pointer_val_val p1))
+     (!! field_compatible node_type [] (pointer_val_val p2) &&
+        EX v: reptype node_type, data_at sh node_type v (pointer_val_val p2)).
+    - apply exp_left; intros [[d l] r]; normalize.
+      apply (exp_right (repinj node_type (d, (l, r)))).
+      rewrite andp_comm, <- (add_andp _ _ (data_at_compatible _ _ _ _)).
+      apply derives_refl.
+    - apply exp_left; intros [[d l] r]; normalize.
+      apply (exp_right (repinj node_type (d, (l, r)))).
+      rewrite andp_comm, <- (add_andp _ _ (data_at_compatible _ _ _ _)).
+      apply derives_refl.
+    - apply disj_prop_andp_left; [apply field_compatible_dec | intro].
+      apply disj_prop_andp_right; [apply field_compatible_dec | intro].
+      apply disj_data_at.
+      change (sizeof cenv_cs node_type) with 16.
+      unfold addr_eqb in H; simpl in H.
+      destruct (PV_eq_dec p1 p2); [congruence |].
+      destruct H0 as [? [_ [_ [_ [_ [_ [? _]]]]]]].
+      destruct H1 as [? [_ [_ [_ [_ [_ [? _]]]]]]].
+      unfold align_compatible in *.
+      change (alignof cenv_cs node_type) with 16 in *.
+      destruct p1, p2;
+        try solve [simpl in H0; tauto | simpl in  H1; tauto].
+      cbv beta iota zeta delta [pointer_val_val] in *; clear H0 H1.
+      intros [[? ?] [[? ?] [? [? ?]]]].
+      inv H0; inv H1.
+      apply res_predicates.range_overlap_spec in H4; [| omega | omega].
+      assert (Int.unsigned i = Int.unsigned i0) by (destruct H4 as [[? ?] | [? ?]], H3, H2; omega).
+      assert (b = b0) by (destruct H4 as [[? ?] | [? ?]]; subst; auto).
+      apply n.
+      rewrite H1, <- (Int.repr_unsigned i), H0, Int.repr_unsigned; auto.
+Defined.
+
+Instance SGA_VST (sh: Share.t) : SpatialGraphAssum.
+  apply (Build_SpatialGraphAssum mpred _ _ _ _ _ _ _ _ SGS_VST (trinode sh) _ (sMSLstandard sh)).
+Defined.
+
 
