sample_mark/mark.v
@@ -63,9 +63,9 @@ Definition f_mark := {|
   fn_callconv := cc_default;
   fn_params := ((_x, (tptr (Tstruct _Node noattr))) :: nil);
   fn_vars := nil;
-  fn_temps := ((_l, (tptr (talignas 4%N (Tstruct _Node noattr)))) ::
-               (_r, (tptr (talignas 4%N (Tstruct _Node noattr)))) ::
-               (_root_mark, tint) :: nil);
+  fn_temps := ((_l, (tptr (Tstruct _Node noattr))) ::
+               (_r, (tptr (Tstruct _Node noattr))) :: (_root_mark, tint) ::
+               nil);
   fn_body :=
 (Ssequence
   (Sifthenelse (Ebinop Oeq (Etempvar _x (tptr (Tstruct _Node noattr)))
@@ -76,7 +76,7 @@ Definition f_mark := {|
     (Sset _root_mark
       (Efield
         (Ederef (Etempvar _x (tptr (Tstruct _Node noattr)))
-          (Tstruct _Node noattr)) _m tint))
+          (Tstruct _Node noattr)) _m (talignas 4%N tint)))
     (Ssequence
       (Sifthenelse (Ebinop Oeq (Etempvar _root_mark tint)
                      (Econst_int (Int.repr 1) tint) tint)
@@ -87,44 +87,41 @@ Definition f_mark := {|
           (Efield
             (Ederef (Etempvar _x (tptr (Tstruct _Node noattr)))
               (Tstruct _Node noattr)) _l
-            (tptr (talignas 4%N (Tstruct _Node noattr)))))
+            (talignas 3%N (tptr (Tstruct _Node noattr)))))
         (Ssequence
           (Sset _r
             (Efield
               (Ederef (Etempvar _x (tptr (Tstruct _Node noattr)))
-                (Tstruct _Node noattr)) _r
-              (tptr (talignas 4%N (Tstruct _Node noattr)))))
+                (Tstruct _Node noattr)) _r (tptr (Tstruct _Node noattr))))
           (Ssequence
             (Sassign
               (Efield
                 (Ederef (Etempvar _x (tptr (Tstruct _Node noattr)))
-                  (Tstruct _Node noattr)) _m tint)
+                  (Tstruct _Node noattr)) _m (talignas 4%N tint))
               (Econst_int (Int.repr 1) tint))
             (Ssequence
               (Scall None
                 (Evar _mark (Tfunction
                               (Tcons (tptr (Tstruct _Node noattr)) Tnil)
                               tvoid cc_default))
-                ((Etempvar _l (tptr (talignas 4%N (Tstruct _Node noattr)))) ::
-                 nil))
+                ((Etempvar _l (tptr (Tstruct _Node noattr))) :: nil))
               (Scall None
                 (Evar _mark (Tfunction
                               (Tcons (tptr (Tstruct _Node noattr)) Tnil)
                               tvoid cc_default))
-                ((Etempvar _r (tptr (talignas 4%N (Tstruct _Node noattr)))) ::
-                 nil)))))))))
+                ((Etempvar _r (tptr (Tstruct _Node noattr))) :: nil)))))))))
 |}.
 
 Definition v_hd := {|
-  gvar_info := (tptr (talignas 4%N (Tstruct _Node noattr)));
+  gvar_info := (tptr (Tstruct _Node noattr));
   gvar_init := (Init_space 4 :: nil);
   gvar_readonly := false;
   gvar_volatile := false
 |}.
 
 Definition v_n := {|
-  gvar_info := (talignas 4%N (Tstruct _Node noattr));
-  gvar_init := (Init_space 12 :: nil);
+  gvar_info := (Tstruct _Node noattr);
+  gvar_init := (Init_space 16 :: nil);
   gvar_readonly := false;
   gvar_volatile := false
 |}.
@@ -137,32 +134,31 @@ Definition f_main := {|
   fn_temps := nil;
   fn_body :=
 (Ssequence
-  (Sassign (Evar _hd (tptr (talignas 4%N (Tstruct _Node noattr))))
-    (Eaddrof (Evar _n (talignas 4%N (Tstruct _Node noattr)))
-      (tptr (talignas 4%N (Tstruct _Node noattr)))))
+  (Sassign (Evar _hd (tptr (Tstruct _Node noattr)))
+    (Eaddrof (Evar _n (Tstruct _Node noattr)) (tptr (Tstruct _Node noattr))))
   (Ssequence
-    (Sassign (Efield (Evar _n (talignas 4%N (Tstruct _Node noattr))) _m tint)
+    (Sassign (Efield (Evar _n (Tstruct _Node noattr)) _m (talignas 4%N tint))
       (Econst_int (Int.repr 0) tint))
     (Ssequence
       (Sassign
-        (Efield (Evar _n (talignas 4%N (Tstruct _Node noattr))) _l
-          (tptr (talignas 4%N (Tstruct _Node noattr))))
-        (Evar _hd (tptr (talignas 4%N (Tstruct _Node noattr)))))
+        (Efield (Evar _n (Tstruct _Node noattr)) _l
+          (talignas 3%N (tptr (Tstruct _Node noattr))))
+        (Evar _hd (tptr (Tstruct _Node noattr))))
       (Ssequence
         (Sassign
-          (Efield (Evar _n (talignas 4%N (Tstruct _Node noattr))) _r
-            (tptr (talignas 4%N (Tstruct _Node noattr))))
-          (Econst_int (Int.repr 0) tint))
+          (Efield (Evar _n (Tstruct _Node noattr)) _r
+            (tptr (Tstruct _Node noattr))) (Econst_int (Int.repr 0) tint))
         (Scall None
           (Evar _mark (Tfunction (Tcons (tptr (Tstruct _Node noattr)) Tnil)
                         tvoid cc_default))
-          ((Evar _hd (tptr (talignas 4%N (Tstruct _Node noattr)))) :: nil))))))
+          ((Evar _hd (tptr (Tstruct _Node noattr))) :: nil))))))
 |}.
 
 Definition composites : list composite_definition :=
 (Composite _Node Struct
-   ((_m, tint) :: (_l, (tptr (talignas 4%N (Tstruct _Node noattr)))) ::
-    (_r, (tptr (talignas 4%N (Tstruct _Node noattr)))) :: nil)
+   ((_m, (talignas 4%N tint)) ::
+    (_l, (talignas 3%N (tptr (Tstruct _Node noattr)))) ::
+    (_r, (tptr (Tstruct _Node noattr))) :: nil)
    noattr :: nil).
 
 Definition prog : Clight.program := {|
